warblreequiv/CharDescrCharSet.v
@@ -1,0 +1,39 @@
+From Linden Require Import Chars LindenParameters.
+From Warblre Require Import Parameters.
+
+Definition equiv_cd_charset (cd: char_descr) (charset: CharSet) :=
+  forall c: Char, char_match c cd = CharSet.contains charset c.
+
+(* Lemma for character descriptor inversion *)
+Lemma equiv_cd_inv:
+  forall cd s, equiv_cd_charset cd s -> equiv_cd_charset (CdInv cd) (CharSet.remove_all Characters.all s).
+Proof.
+  intros cd s H c.
+  rewrite charset_remove_all_contains. simpl. specialize (H c).
+  unfold Characters.all, Character.all. simpl. rewrite charset_from_list_contains_inb, char_all_inb. simpl. now f_equal.
+Qed.
+
+(* Lemmas for various character descriptors *)
+Lemma equiv_cd_digits:
+  equiv_cd_charset CdDigits Characters.digits.
+Proof.
+  intro c. simpl. unfold Characters.digits. now rewrite charset_from_list_contains_inb.
+Qed.
+
+Lemma equiv_cd_whitespace:
+  equiv_cd_charset CdWhitespace (CharSet.union Characters.white_spaces Characters.line_terminators).
+Proof.
+  intro c. simpl. unfold Characters.white_spaces, Characters.line_terminators. rewrite charset_union_contains. now do 2 rewrite charset_from_list_contains_inb.
+Qed.
+
+Lemma equiv_cd_wordchar:
+  equiv_cd_charset CdWordChar Characters.ascii_word_characters.
+Proof.
+  intro c. simpl. unfold Characters.ascii_word_characters. now rewrite charset_from_list_contains_inb.
+Qed.
+
+Lemma equiv_cd_single:
+  forall c, equiv_cd_charset (CdSingle c) (CharSet.singleton c).
+Proof.
+  intros c chr. simpl. symmetry. apply charset_contains_singleton.
+Qed.
